Set_Graphs/Graph_Algorithms/BFS_Refinement_2.thy
@@ -1,7 +1,12 @@
 theory BFS_Refinement_2
   imports BFS_3 BFS_Subprocedures  Directed_Set_Graphs.Pair_Graph_Imperative
 "HOL-Imperative_HOL.Imperative_HOL" "HOL-Library.IArray" BFS_Refinement
+CSR_Graph
 begin
+
+lemma triple_res_ht_ex_pre_and_post_I:"(\<And> x. <P x> c <\<lambda> (r1,r2,r3). Q x r1 r2 r3>) 
+           \<Longrightarrow> <\<exists>\<^sub>A x. P x> c <\<lambda> (r1,r2,r3). \<exists>\<^sub>A x. Q x r1 r2 r3>"
+  by sep_auto
 
 lemma "<a \<mapsto>\<^sub>a xs * a' \<mapsto>\<^sub>a xs' * \<up> (i < length xs \<and> j < length xs')>
        do {Array.upd i x a; Array.upd j x' a'}
@@ -13,7 +18,7 @@ record ('imp_dist, 'imp_vis, 'imp_cf) BFS_state_imp =
 
 locale BFS_Imperative_spec = 
 fixes imp_src_to_cf::"'imp_src \<Rightarrow> 'imp_cf Heap"
-and set_srcs_visited::"'imp_src \<Rightarrow> 'imp_vis Heap"
+and set_srcs_visited::" 'imp_vis \<Rightarrow> 'imp_src \<Rightarrow> 'imp_vis Heap"
 and next_frontier_and_current_imp::"'imp_cf \<Rightarrow> 'imp_vis \<Rightarrow> ('imp_cf \<times> 'imp_vis) Heap"
 and imp_cf_is_empty::"'imp_cf \<Rightarrow> bool Heap"
 and in_vis::"'ver \<Rightarrow> 'imp_vis \<Rightarrow> bool Heap"
@@ -32,14 +37,14 @@ partial_function (heap) BFS_dist_imp::
                BFS_dist_imp (state \<lparr>dists:= dist', visited := visited', current := current',
                                  current_dist := Suc d\<rparr>)}}"
 
-definition "initial_state_imp src_imp imp_some_dist=  
-  do {cf \<leftarrow> imp_src_to_cf src_imp;
+definition "initial_state_imp empty_vis src_imp imp_some_dist=  
+  do {v \<leftarrow> set_srcs_visited empty_vis src_imp;
+      cf \<leftarrow> imp_src_to_cf src_imp;
       dists \<leftarrow> set_all_dists_in_front_imp  imp_some_dist cf 0;
-      v \<leftarrow> set_srcs_visited src_imp;
-        return \<lparr>dists = dists, current = cf, visited = v, current_dist = 0\<rparr>}"
+      return \<lparr>dists = dists, current = cf, visited = v, current_dist = 0\<rparr>}"
 
-definition "check_reachable src_imp imp_some_dist t =
-    do {init \<leftarrow> initial_state_imp src_imp imp_some_dist;
+definition "check_reachable empty_vis src_imp imp_some_dist t =
+    do {init \<leftarrow> initial_state_imp empty_vis src_imp imp_some_dist;
         final \<leftarrow> BFS_dist_imp init;
         in_vis t (visited final)}"
 end
@@ -63,17 +68,18 @@ fixes  G_imp::"'imp_G"
 assumes imp_sf_is_empty: "\<And> S Si. <imp_cf_assn S Si> imp_cf_is_empty Si 
                        <\<lambda> b. imp_cf_assn S Si * \<up>(b \<longleftrightarrow> S = \<emptyset>\<^sub>N)>"
  and imp_src_to_cf: "\<And> S Si. <imp_src_assn S Si> imp_src_to_cf Si 
-                      <\<lambda> r. imp_src_assn S Si * imp_cf_assn S r>"
+                      <\<lambda> r. imp_cf_assn S r>"
  and set_srcs_visited: 
   "\<And> S Si. 
-    <imp_src_assn S Si> set_srcs_visited Si  <\<lambda> r. imp_vis_assn S r * imp_src_assn S Si>"
+    <imp_src_assn S Si * imp_vis_assn vset_empty empty_vis> set_srcs_visited empty_vis Si 
+           <\<lambda> r. imp_vis_assn S r * imp_src_assn S Si>"
  and next_frontier_and_current_imp:  "\<And> cf imp_cf vis imp_vis.
     <imp_cf_assn cf imp_cf * imp_vis_assn vis imp_vis * graph_assn G G_imp>
     next_frontier_and_current_imp imp_cf imp_vis
     <\<lambda> (r1, r2). imp_cf_assn (fst (next_frontier_and_current cf vis)) r1 * 
                  imp_vis_assn (snd (next_frontier_and_current cf vis)) r2 * graph_assn G G_imp>"
-and in_vis_rule: "\<And>vis visi s. <imp_vis_assn vis visi> in_vis s visi 
-            <\<lambda> r. imp_vis_assn vis visi * \<up> (r \<longleftrightarrow> isin vis s)>"
+(*and in_vis_rule: "\<And>vis visi s. <imp_vis_assn vis visi> in_vis s visi 
+            <\<lambda> r. imp_vis_assn vis visi * \<up> (r \<longleftrightarrow> isin vis s)>"*)
 and set_all_dists_in_front_imp:
     "\<And> d id. <imp_dist_assn d id * imp_cf_assn cf cfi> set_all_dists_in_front_imp id cfi n
             <\<lambda> r. imp_dist_assn (set_all_dists_in_set d cf n) r * imp_cf_assn cf cfi>"
@@ -119,38 +125,360 @@ next
 qed
 
 lemma initial_refine:
- "<imp_src_assn srcs srcs_imp * imp_dist_assn some_dist imp_some_dist>
-  initial_state_imp srcs_imp imp_some_dist
- <\<lambda> si. state_assn initial_dist_state si * imp_src_assn srcs srcs_imp>"
+ "<imp_vis_assn vset_empty empty_vis* imp_src_assn srcs srcs_imp * imp_dist_assn some_dist imp_some_dist>
+  initial_state_imp empty_vis srcs_imp imp_some_dist
+ <\<lambda> si. state_assn initial_dist_state si>"
   apply(auto simp add: initial_dist_state_def state_assn_def initial_state_imp_def)
   using imp_src_to_cf set_all_dists_in_front_imp set_srcs_visited 
   by sep_auto
 
 lemma BFS_program_behaviour:
-  "<imp_src_assn srcs srcs_imp * imp_dist_assn some_dist imp_some_dist * graph_assn G G_imp>
-   do { si \<leftarrow> initial_state_imp srcs_imp imp_some_dist;
+  "<imp_vis_assn vset_empty empty_vis * imp_src_assn srcs srcs_imp * imp_dist_assn some_dist imp_some_dist * graph_assn G G_imp>
+   do { si \<leftarrow> initial_state_imp empty_vis srcs_imp imp_some_dist;
         BFS_dist_imp si }
-   < \<lambda> si'. state_assn (BFS_dist_impl initial_dist_state) si' * imp_src_assn srcs srcs_imp * graph_assn G G_imp>"
+   < \<lambda> si'. state_assn (BFS_dist_impl initial_dist_state) si' * graph_assn G G_imp>"
   using initial_refine BFS_refine 
   by sep_auto
 
 lemma check_reachable_rule:
- "<imp_src_assn srcs srcs_imp * imp_dist_assn some_dist imp_some_dist * graph_assn G G_imp> 
-   check_reachable srcs_imp imp_some_dist t
-  <\<lambda> b. imp_src_assn srcs srcs_imp * graph_assn G G_imp *
+ "<imp_vis_assn vset_empty empty_vis * imp_src_assn srcs srcs_imp * imp_dist_assn some_dist imp_some_dist * graph_assn G G_imp> 
+   check_reachable empty_vis srcs_imp imp_some_dist t
+  <\<lambda> b.  graph_assn G G_imp *
       \<up> (b \<longleftrightarrow> isin (BFS_dist_state.visited (BFS_dist_impl initial_dist_state)) t)>" 
   unfolding check_reachable_def
   using initial_refine BFS_refine in_vis_rule
   by (sep_auto simp: state_assn_def)
 end
 
+locale imp_fixed_univ_set =
+  fixes is_fixed_univ_set :: "'a set \<Rightarrow> 'a set \<Rightarrow> 's \<Rightarrow> assn"
+  assumes only_in_univ: "is_fixed_univ_set U S Si = (is_fixed_univ_set U S Si * \<up> (S \<subseteq> U))"
+(*
+locale imp_set_empty = imp_set +
+  constrains is_set :: "'a set \<Rightarrow> 'a set \<Rightarrow> 's \<Rightarrow> assn"
+  fixes empty :: "'s Heap"
+  and U::"'a set"
+  assumes empty_rule[sep_heap_rules]: "<emp> empty <is_set {}>"
+*)(*
+locale imp_fixed_univ_set_is_empty = imp_fixed_univ_set +
+  constrains is_fixed_univ_set :: "'a set \<Rightarrow> 'a set \<Rightarrow> 's \<Rightarrow> assn"
+  fixes is_empty :: "'s \<Rightarrow> bool Heap"
+  assumes is_empty_rule[sep_heap_rules]: 
+    "<is_fixed_univ_set U s p> is_empty p <\<lambda>r. is_fixed_univ_set U s p * \<up>(r \<longleftrightarrow> s={})>"
+*)
+locale imp_fixed_univ_set_memb = imp_fixed_univ_set +
+  constrains is_fixed_univ_set :: "'a set \<Rightarrow> 'a set \<Rightarrow> 's \<Rightarrow> assn"
+  fixes memb :: "'a \<Rightarrow> 's \<Rightarrow> bool Heap"
+  assumes memb_rule[sep_heap_rules]: 
+    "<is_fixed_univ_set U s p * \<up> (a \<in> U)> memb a p <\<lambda>r. is_fixed_univ_set U s p * \<up>(r \<longleftrightarrow> a \<in> s)>"
+
+locale imp_fixed_univ_set_ins = imp_fixed_univ_set +
+  constrains is_fixed_univ_set :: "'a set \<Rightarrow> 'a set \<Rightarrow> 's \<Rightarrow> assn"
+  fixes ins :: "'a \<Rightarrow> 's \<Rightarrow> 's Heap"
+  assumes ins_rule[sep_heap_rules]: 
+    "<is_fixed_univ_set U s p * \<up> (a \<in> U)> ins a p <is_fixed_univ_set U (Set.insert a s)>"
+
+locale imp_fixed_univ_set_distinct_ins = imp_fixed_univ_set +
+  constrains is_fixed_univ_set :: "'a set \<Rightarrow> 'a set \<Rightarrow> 's \<Rightarrow> assn"
+  fixes distinct_ins :: "'a \<Rightarrow> 's \<Rightarrow> 's Heap"
+  assumes distinct_ins_rule[sep_heap_rules]: 
+    "<is_fixed_univ_set U s p * \<up> (a \<in> U \<and> a \<notin> s)> distinct_ins a p <is_fixed_univ_set U (Set.insert a s)>"
+
+locale imp_fixed_univ_set_rest = imp_fixed_univ_set +
+  constrains is_fixed_univ_set :: "'a set \<Rightarrow> 'a set \<Rightarrow> 's \<Rightarrow> assn"
+  fixes reset :: "'s \<Rightarrow> 's Heap"
+  assumes ins_rule[sep_heap_rules]: 
+    "<is_fixed_univ_set U s p > reset p <is_fixed_univ_set U {}>"
+  
+
 locale BFS_subprocedures_lists =
-  fixes G::"'a \<Rightarrow> 'a list option"
+  imp_fixed_univ_set_memb where is_fixed_univ_set = is_visited_set
+  and memb = visited_memb +
+  imp_fixed_univ_set_distinct_ins where is_fixed_univ_set = is_visited_set
+for is_visited_set and visited_memb::"nat \<Rightarrow> 'imp_vis \<Rightarrow> bool Heap"
 begin
+
+definition "Vs (G::nat \<Rightarrow> nat list option) = \<Union> {{u, v} | u v vs. G u = Some vs \<and> v \<in> set vs }"
+
+fun inner_loop where
+"inner_loop Gi sindicesi eindicesi u (front, frontpt, vis) =
+   iterate_neighbourhood Gi sindicesi eindicesi u 
+     (\<lambda> u v (front, frontpt, vis) . 
+          do {b \<leftarrow> visited_memb v vis;
+              if \<not> b then do { front' \<leftarrow> Array.upd frontpt v front;
+                               vis' \<leftarrow> distinct_ins v vis;
+                               return (front', Suc frontpt, vis')}
+              else return (front, frontpt, vis)})
+      (front, frontpt, vis)"
+
+definition "front_assn G vis (front::nat list) fronti frontp = 
+  (\<exists>\<^sub>A frontlist. fronti \<mapsto>\<^sub>a frontlist * \<up> (length frontlist > card (Vs G) \<and>
+     frontp < length frontlist - card (Vs G) + card vis \<and> frontp \<le> length frontlist \<and>
+        rev (take frontp (frontlist)) = front
+     \<and> vis \<subseteq> (Vs G) \<and> set front \<subseteq> (Vs G)))"
+
+lemma inner_loop_rule:
+  assumes "(front', vis') = 
+          foldl (\<lambda>x y. case x of (nf, vis) \<Rightarrow> if y \<notin> set vis then (y # nf, y # vis) else (nf, vis))
+            (front, vis) (case G u of None \<Rightarrow> [] | Some ys \<Rightarrow> ys)"
+          "finite (Vs G)"
+  shows "<CSR_assn_raw G Gi sindicesi eindicesi nha sindices eindices
+          * is_visited_set (Vs G) (set vis) visi * front_assn G (set vis) front fronti frontp>
+  inner_loop Gi sindicesi eindicesi u (fronti, frontp, visi)
+ <\<lambda> (fronti', frontp', visi'). 
+   CSR_assn_raw G Gi sindicesi eindicesi nha sindices eindices
+       * is_visited_set (Vs G) (set vis') visi' * front_assn G (set vis') front' fronti' frontp'>"
+proof-
+  define acc_assn where 
+    "acc_assn = (\<lambda> (front, vis) (fronti, frontp, visi). 
+        is_visited_set (Vs G) (set vis) visi * front_assn G (set vis) front fronti frontp)"
+  define fi where "fi = (\<lambda> (u::nat) (v::nat) (front, frontpt, vis) . 
+          do {b \<leftarrow> visited_memb v vis;
+              if \<not> b then do { front' \<leftarrow> Array.upd frontpt v front;
+                               vis' \<leftarrow> distinct_ins v vis;
+                               return (front', Suc frontpt, vis')}
+              else return (front, frontpt, vis)})"
+  define f where "f = (\<lambda>(nf, vis) y. if (y::nat) \<notin> set vis then (y # nf, y # vis) else (nf, vis))"
+  have assms_1': "(front', vis') = 
+          foldl f (front, vis) (case G u of None \<Rightarrow> [] | Some ys \<Rightarrow> ys)"
+    using assms(1) by(auto simp add: f_def case_prod_unfold)
+  show ?thesis
+    unfolding inner_loop.simps fi_def[symmetric]
+    apply(rule ht_cons_prec)
+      defer
+      defer
+      apply(rule iterate_neighbourhood_raw_rule[where F = emp and acc_assn = acc_assn, simplified, of _ _ fi,
+          where nhlists = G and nha = nha and sindices = sindices and eindices = eindices
+           and acc = "(front, vis)" and f = "\<lambda> x. f"])
+    subgoal for acc acci x vs
+    proof(cases acc, cases acci, goal_cases)
+      case (1 front vis fronti frontp visi)
+      have x_in_Vs: "x \<in> (Vs G)" 
+        using 1(1,2)
+        by(auto simp add: Vs_def)
+      show ?case 
+        unfolding 1
+        unfolding acc_assn_def front_assn_def
+        unfolding acc_assn_def f_def fi_def 
+        unfolding prod.case front_assn_def ex_assn_move_out(2)
+      proof(cases "x \<notin> set vis", goal_cases)
+        case 1
+        show ?case
+          apply(subst (2) if_P)
+           using 1 apply force
+           unfolding prod.case 
+           using x_in_Vs apply sep_auto
+           subgoal 
+             by (smt (verit, ccfv_SIG) Nat.add_diff_assoc2 assms(2) card_mono card_seteq le_add_diff_inverse2 le_trans
+                 nat_add_left_cancel_le nat_less_le x_in_Vs)
+           subgoal for h xa ha r hb ra
+             using distinct_ins_rule[of "(Vs G)" "set vis" visi x] x_in_Vs apply sep_auto
+               apply(rule mod_exI[of _ "xa[frontp := x]"])
+               apply (sep_auto simp: mod_pure_star_dist)
+               apply(subst take_Suc_conv_app_nth)
+                apply simp
+             by (metis take_Suc_conv_app_nth take_update_last)
+           subgoal for h xa ha r
+             apply sep_auto
+             apply(rule mod_exI[of _ "xa"])
+             apply sep_auto
+             using "1" by blast
+           done
+       next
+         case 2
+         thus ?case
+           by sep_auto
+       qed
+     qed
+     subgoal
+       unfolding acc_assn_def prod.case 
+       by sep_auto
+     subgoal for x
+       apply(clarsimp split!: option.split prod.split)
+       subgoal for front frontpt vis
+         unfolding acc_assn_def front_assn_def prod.case ex_assn_move_out(2)
+         apply(rule matr.impl_of_exes_assn)
+         using assms(1)
+         by sep_auto
+       subgoal for vs front frontpt vis
+         unfolding acc_assn_def front_assn_def prod.case
+         apply(clarsimp split!: option.split prod.split)
+         subgoal for front' vis'
+           unfolding ex_assn_move_out(2)
+           apply(rule matr.impl_of_exes_assn)
+           using assms_1' 
+           by sep_auto
+         done
+       done
+     done
+ qed
+
+fun outer_loop where
+  "outer_loop Gi sindicesi eindicesi (old_front, old_frontp) (front, frontpt, vis) = 
+    do{iterate_range_strict old_front 0 old_frontp 
+             (inner_loop Gi sindicesi eindicesi) (front, frontpt, vis)}"
+
+definition "old_front_assn G (front::nat list) fronti frontp = 
+  (\<exists>\<^sub>A frontlist. 
+    fronti \<mapsto>\<^sub>a frontlist * \<up> ( frontp < length frontlist \<and> rev (take frontp (frontlist)) = front
+    \<and> card (Vs G) < length frontlist))"
+
+lemma outer_loop_rule:
+  assumes "(front', vis') = 
+   foldl (\<lambda>(nf, vis) u. 
+       foldl (\<lambda>x y. case x of (nf, vis) \<Rightarrow> if y \<notin> set vis then (y # nf, y # vis) else (nf, vis))
+            (nf, vis) (case G u of None \<Rightarrow> [] | Some ys \<Rightarrow> ys)) 
+   (front, vis) (rev old_front)"
+          "finite (Vs G)"
+  shows "<CSR_assn_raw G Gi sindicesi eindicesi nha sindices eindices
+          * is_visited_set (Vs G) (set vis) visi * front_assn G (set vis) front fronti frontp
+          * old_front_assn G old_front old_fronti old_frontp>
+  outer_loop Gi sindicesi eindicesi (old_fronti, old_frontp) (fronti, frontp, visi)
+ <\<lambda> (fronti', frontp', visi'). 
+   CSR_assn_raw G Gi sindicesi eindicesi nha sindices eindices
+       * is_visited_set (Vs G) (set vis') visi' * front_assn G (set vis') front' fronti' frontp'
+       * old_front_assn G old_front old_fronti old_frontp>"
+proof-
+  define acc_assn where 
+    "acc_assn = (\<lambda> (front, vis) (fronti, frontp, visi). 
+        is_visited_set (Vs G) (set vis) visi * front_assn G (set vis) front fronti frontp)"
+  define f where "f = (\<lambda>  (nf, vis) u. foldl (\<lambda>x y. case x of (nf, vis) \<Rightarrow> if y \<notin> set vis then (y # nf, y # vis) else (nf, vis))
+            (nf, vis) (case G u of None \<Rightarrow> [] | Some ys \<Rightarrow> ys))"
+  show ?thesis
+    unfolding outer_loop.simps 
+    unfolding old_front_assn_def ex_assn_move_out(2)
+    apply(rule triple_res_ht_ex_pre_and_post_I)
+    subgoal for old_front_list
+    apply(rule ht_cons_prec)
+      defer
+    defer
+      apply(rule iterate_range_strict_rule[of old_front_list 0 old_frontp acc_assn 
+          "CSR_assn_raw G Gi sindicesi eindicesi nha sindices eindices 
+           * \<up> (old_frontp < length old_front_list \<and> rev (take old_frontp (old_front_list)) = old_front
+                \<and> card (Vs G) < length old_front_list)" 
+           "inner_loop Gi sindicesi eindicesi" f old_fronti "(front, vis)" "(fronti, frontp, visi)"
+             ])
+    subgoal for acc acci x
+      apply(clarsimp simp add: acc_assn_def split: prod.split simp del: inner_loop.simps)
+      subgoal for front vis front' vis' fronit' frontp visi'
+        apply(rule ht_cons_prec)
+        defer defer
+        apply(rule ht_frame[OF inner_loop_rule[of front' vis' front vis G _ _ _ _  nha sindices eindices],
+              where R = "\<up> (old_frontp < length old_front_list \<and> 
+                rev (take old_frontp (old_front_list)) = old_front \<and>
+                   card (Vs G) < length old_front_list)"])
+        by(sep_auto simp: f_def assms(2))
+      done
+      using assms(1)
+      by(sep_auto split: prod.split simp: old_front_assn_def acc_assn_def f_def nths_intervall_strict_as_drop_and_take)
+  
+      done
+qed
+
+fun imp_cf_assn where 
+   "imp_cf_assn (G::nat \<Rightarrow> nat list option) front (fronti, frontp, buffer_fronti) =
+      (\<exists>\<^sub>A frontlist buffer_frontlist. fronti \<mapsto>\<^sub>a frontlist *  buffer_fronti \<mapsto>\<^sub>a buffer_frontlist *
+       \<up> (length frontlist > card (Vs G) \<and> frontp < length frontlist  \<and> 
+          rev (take frontp (frontlist)) = front \<and> length buffer_frontlist > card (Vs G)
+          \<and> set front \<subseteq> (Vs G)))"
+
+definition "imp_src_to_cf = (\<lambda> x. return x)"
+definition "imp_src_assn = imp_cf_assn"
+
+fun imp_cf_is_empty where
+ "imp_cf_is_empty (fronti, frontp, buffer_fronti) = 
+          return (frontp = 0)"
+
+lemma imp_cf_is_empty_rule:
+  "<imp_cf_assn G S Si> imp_cf_is_empty Si <\<lambda>b. imp_cf_assn G S Si * \<up> (b = (S = []))>"
+  by(cases Si) sep_auto
+term inner_loop
+
+fun set_srcs_visited where
+  "set_srcs_visited (imp_vis::'imp_vis) (fronti, frontp, buffer_fronti) =
+   do { iterate_range_strict fronti 0 frontp 
+             (\<lambda> v vis. do {b \<leftarrow> visited_memb v vis;
+                           if \<not> b then distinct_ins v vis
+                           else return vis})
+             imp_vis}"
+
+lemma foldl_insert:"foldl (\<lambda>S x. if x \<in> S then S else Set.insert x S) A xs = set xs \<union> A"
+  by(induction xs arbitrary: A) auto
+
+lemma set_srcs_visited_rule:
+      "<imp_src_assn G S Si * is_visited_set (Vs G) {} empty_vis> 
+          set_srcs_visited empty_vis Si
+        <\<lambda>r. is_visited_set (Vs G) (set S) r * imp_src_assn G S Si>"
+  unfolding imp_src_assn_def
+  apply(cases Si)
+  subgoal for fronti frontp buffer_fronti
+    apply simp
+    apply(rule ht_ex_pre_and_post_I)+
+    subgoal for frontlist buffer_frontlist
+  apply(rule ht_cons_prec)
+      defer defer
+        apply(rule iterate_range_strict_rule[where acc_assn = "is_visited_set (Vs G)"
+             and F = "buffer_fronti \<mapsto>\<^sub>a buffer_frontlist *
+    \<up> (card (Vs G) < length frontlist \<and>
+       frontp < length frontlist \<and> rev (take frontp frontlist) = S \<and> card (Vs G) < length buffer_frontlist \<and> set S \<subseteq> Vs G)"
+         and f = "\<lambda> S x. if x \<notin> S then Set.insert x S else S" and list = frontlist and acc = Set.empty])
+     by (sep_auto simp: foldl_insert nths_intervall_strict_as_drop_and_take)
+   done
+  done
+
+abbreviation "imp_dist_assn_raw G dlist d di 
+   \<equiv> (di \<mapsto>\<^sub>a dlist * 
+          \<up>((\<forall> i \<in> dom G. i < length dlist \<and> d i = dlist ! i)))"
+
+definition "imp_dist_assn G d di 
+   = (\<exists>\<^sub>A dlist. di \<mapsto>\<^sub>a dlist * 
+          \<up>((\<forall> i \<in> Vs G. i < length dlist \<and> d i = dlist ! i)))"
+
+fun set_all_dists_in_front_imp where
+ "set_all_dists_in_front_imp di (fronti, frontp, buffer_fronti) n = 
+       iterate_range_strict fronti 0 frontp 
+         (\<lambda> v di. Array.upd v n di) di"
+
+lemma foldl_fun_upd_same: "foldl (\<lambda>d x y. if x = y then n else d y) d xs =
+       (\<lambda> x. if x \<in> set xs then n else d x)"
+  by(induction xs arbitrary: d)  auto
+
+lemma set_all_dists_in_front_imp_rule:
+  "<imp_dist_assn G d di * imp_cf_assn G cf cfi> set_all_dists_in_front_imp di cfi n
+    <\<lambda>r. imp_dist_assn G (\<lambda>y. if y \<in> set cf then n else d y) r * imp_cf_assn G cf cfi>"
+  apply(cases cfi)
+  subgoal for fronti frontp buffer_fronti
+    apply simp 
+    apply(rule ht_ex_pre_and_post_I)+
+    subgoal for frontlist buffer_frontlist
+    apply(rule ht_cons_prec)
+      defer defer
+        apply(rule iterate_range_strict_rule[where list = frontlist
+               and acc_assn = "imp_dist_assn G" and acc = d
+               and F = "buffer_fronti \<mapsto>\<^sub>a buffer_frontlist *
+          \<up> (card (Vs G) < length frontlist \<and> frontp < length frontlist \<and>
+        rev (take frontp frontlist) = cf \<and> card (Vs G) < length buffer_frontlist \<and> set cf \<subseteq> Vs G)"
+               and f = "\<lambda> d. \<lambda> x y. if x = y then n else d y"])
+      by (sep_auto simp: imp_dist_assn_def nths_intervall_strict_as_drop_and_take 
+         nths_intervall_strict_as_drop_and_take foldl_fun_upd_same)
+    done
+  done
+
+fun next_frontier_and_current_imp where
+  "next_frontier_and_current_imp Gi sindicesi eindicesi (fronti, frontp, buffer_fronti) imp_vis =
+   do{
+      (front', frontpt', vis') \<leftarrow> 
+       outer_loop Gi sindicesi eindicesi (fronti, frontp) (buffer_fronti, 0, imp_vis);
+      return ((front', frontpt', fronti), vis')}"
+
+lemma verts_rw:
+   "\<Union> {{v1, v2} |v1 v2. (v1, v2) \<in> {(u, v). v \<in> set (case G u of None \<Rightarrow> [] | Some vset \<Rightarrow> vset)}} =
+    \<Union> {uu. \<exists>u v vs. uu = {u, v} \<and> G u = Some vs \<and> v \<in> set vs}"
+  by auto (metis insert_iff)+
 
 sublocale BFS_subprocedures_3
   where empty = "\<lambda> x. None"
-  and delete = "\<lambda> x M. \<lambda> y. if y = x then None else M y"
+  and delete = "\<lambda> (x::nat) M. \<lambda> y. if y = x then None else M y"
   and insert = Cons
   and isin = "\<lambda> xs x. x \<in> set xs"
   and t_set = set
@@ -167,14 +495,263 @@ sublocale BFS_subprocedures_3
   and fold_adjmap = "\<lambda>  f xs a. foldl (\<lambda>x y. f y x) a xs"
   and lookup = "\<lambda> M x. M x"
   and fold2_vset = "\<lambda>  f xs a. foldl (\<lambda>x y. f y x) a xs"
+  and fold2_vset' = "\<lambda>  f xs a. foldl (\<lambda>x y. f y x) a (rev xs)"
   and fast_insert = Cons
   and vset_inv2 = distinct
   apply unfold_locales
-  by (auto intro: exI[of _ "rev _"] simp add: foldl_conv_foldr) 
+  apply (auto intro: exI[of _ "rev _"] simp add: foldl_conv_foldr) 
+  done
 
 
-thm next_frontier_and_curent_correct
+lemma next_frontier_and_current_imp_rule:
+  fixes G::"nat \<Rightarrow> nat list option"
+  assumes "finite (Vs G)" "G_imp = Gi" 
+  shows 
+    "<imp_cf_assn G cf imp_cf * is_visited_set (Vs G) (set vis) imp_vis *
+     CSR_assn_raw G G_imp sindicesi eindicesi nha sindices eindices>
+    next_frontier_and_current_imp Gi sindicesi eindicesi imp_cf imp_vis
+    <\<lambda>(r1, r2).
+        imp_cf_assn G (fst (next_frontier_and_current cf vis)) r1 *
+        is_visited_set (Vs G) (set (snd (next_frontier_and_current cf vis))) r2 *
+        CSR_assn_raw G G_imp sindicesi eindicesi nha sindices eindices>"
+proof(cases imp_cf, cases "next_frontier_and_current cf vis", goal_cases)
+  case (1 fronti frontp buffer_fronti cf' vis')
+  show ?case
+    unfolding 1 fst_conv snd_conv next_frontier_and_current_imp.simps
+    apply(rule ht_bind[where R = "\<lambda> x. (case x of
+          (fronti', frontp', visi') \<Rightarrow>
+            CSR_assn_raw G Gi sindicesi eindicesi nha sindices eindices * is_visited_set (Vs G) (set vis') visi' *
+            front_assn G (set vis') cf' fronti' frontp' *
+            old_front_assn G cf fronti frontp)"])
+    apply(rule ht_cons_prec)
+    defer defer
+    apply(rule outer_loop_rule[of cf' vis' G Nil vis cf _ _  _ nha sindices eindices, OF _ assms(1)])
+    subgoal
+      unfolding 1(2)[symmetric] next_frontier_and_current_def Graph.neighbourhood_def 
+      apply(rule fun_cong[of "foldl _ _" "foldl _ _"])
+      apply(rule fun_cong[of "foldl _" "foldl _"])
+      apply(rule arg_cong[of _ _ foldl])
+      by fast
+      defer
+    subgoal
+      apply (sep_auto intro: simp: front_assn_def old_front_assn_def)
+      apply(rule matr.impl_of_exes_assn)+
+      subgoal for frontlist buffer_frontlist
+      apply(subst only_in_univ)
+        apply(subst ent_pure_pre_iff)+
+        apply rule
+        apply(subst ent_pure_post_iff)+
+      apply rule+
+        subgoal
+          unfolding assms(2)
+          apply(elim conjE)
+          by (metis  ent_refl  assms(2) only_in_univ  star_aci(2) star_aci(3))
+        subgoal
+          apply rule+
+          subgoal 
+            by auto
+          subgoal
+            by (metis mod_false pure_false star_false_left star_false_right)
+          done
+        subgoal
+          by sep_auto
+        done
+      done
+    subgoal
+      by sep_auto
+    subgoal for x
+    proof(cases x, goal_cases)
+      case (1 fronti' frontpt' visi' )
+      show ?case 
+        unfolding 1 prod.case
+        apply(rule ht_cons_post_prec)
+        apply(rule ht_return_sp)
+        apply (sep_auto )
+        unfolding front_assn_def ex_assn_move_out old_front_assn_def
+        apply(rule ent_ex_preI)+
+        subgoal for frontlist buffer_frontlist
 
+          apply(rule ent_ex_postI[of _ _ buffer_frontlist])
+          apply(rule ent_ex_postI[of _ _ frontlist])
+        proof(goal_cases)
+          case 1
+          have assn_rw:"CSR_assn_raw G Gi sindicesi eindicesi nha sindices eindices * is_visited_set (Vs G) (set vis') visi' *
+    (fronti' \<mapsto>\<^sub>a buffer_frontlist *
+     \<up> (card (Vs G)< length buffer_frontlist \<and>
+        frontpt' < length buffer_frontlist - card (Vs G) + card (set vis') \<and>
+        frontpt' \<le> length buffer_frontlist \<and> rev (take frontpt' buffer_frontlist) = cf' \<and> set vis' \<subseteq> (Vs G)
+         \<and> set cf' \<subseteq> (Vs G))) *
+    (fronti \<mapsto>\<^sub>a frontlist *
+     \<up> (frontp < length frontlist \<and> rev (take frontp frontlist) = cf \<and> card (Vs G) < length frontlist)) = 
+       CSR_assn_raw G Gi sindicesi eindicesi nha sindices eindices * is_visited_set (Vs G) (set vis') visi' *
+  fronti' \<mapsto>\<^sub>a buffer_frontlist * fronti \<mapsto>\<^sub>a frontlist *
+   \<up> (card (Vs G) < length buffer_frontlist \<and>
+        frontpt' < length buffer_frontlist - card (Vs G) + card (set vis') \<and>
+        frontpt' \<le> length buffer_frontlist \<and> rev (take frontpt' buffer_frontlist) = cf' \<and> set vis' \<subseteq> (Vs G) 
+        \<and> set cf' \<subseteq> (Vs G) \<and>
+         frontp < length frontlist \<and> rev (take frontp frontlist) = cf \<and> card (Vs G) < length frontlist)"
+            by (smt (verit, best) merge_pure_star mult_left_assoc star_aci(3))
+        
+          show ?case
+           apply(insert 1)
+            unfolding assn_rw ent_pure_pre_iff ent_pure_post_iff
+            apply rule+
+            subgoal
+              unfolding assms(2)
+              by (metis ent_refl star_aci(3) star_aci(2))
+            using assms(1) card_mono[of "(Vs G)" "set vis'"] 
+            by (auto simp: mod_pure_star_dist)
+        qed
+        done
+    qed
+    done
+qed
 
+lemma Vs_same:"dVs (Graph.digraph_abs G) =  Vs G"
+  unfolding Vs_def Graph.digraph_abs_def Graph.neighbourhood_def dVs_def verts_rw[of G]
+  by order
+
+context fixes nha sindices eindices ::"nat list"
+and Gi sindicesi eindicesi::"nat array"
+assumes finite_Vs:"finite (Vs G)"
+begin
+
+interpretation imp_bfs: BFS_Imperative
+where empty = "\<lambda> x. None"
+  and delete = "\<lambda> x M. \<lambda> y. if y = x then None else M y"
+  and insert = Cons
+  and isin = "\<lambda> xs x. x \<in> set xs"
+  and t_set = set
+  and sel = hd
+  and  update = "\<lambda> x z M. \<lambda> y. if y = x then Some z else M y"
+  and adjmap_inv = "\<lambda> _. True"
+  and vset_empty = Nil
+  and vset_delete = "\<lambda> x xs. filter (\<lambda> y. x \<noteq> y) xs"
+  and vset_inv = "\<lambda> _. True"
+  and union = append
+  and inter = "\<lambda> xs ys. filter (\<lambda> y. y \<in> set ys) xs"
+  and diff = "\<lambda> xs ys. filter (\<lambda> y. y \<notin> set ys) xs"
+  and lookup = "\<lambda> M x. M x"
+  and vset_inv2 = distinct
+  and G = G
+  and next_frontier_and_current = next_frontier_and_current
+and next_frontier_and_current_imp = "next_frontier_and_current_imp Gi sindicesi eindicesi"
+and imp_cf_assn = "imp_cf_assn G"
+and expand_tree = expand_tree
+and graph_assn = "\<lambda> G Gi. CSR_assn_raw G Gi sindicesi eindicesi nha sindices eindices"
+and imp_vis_assn = "\<lambda> xs. is_visited_set (Vs G) (set xs)"
+and G_imp = Gi
+and imp_cf_is_empty = imp_cf_is_empty
+and imp_src_assn = "imp_src_assn G"
+and imp_src_to_cf = imp_src_to_cf
+and set_srcs_visited = set_srcs_visited
+and in_vis = visited_memb
+and dist_invar = "\<lambda> d S. S \<subseteq> (Vs G)"
+and dist_lookup = "\<lambda> d x. d x"
+and set_all_dists_in_set = "\<lambda> d S n. \<lambda> y. if y \<in> set S then n else d y"
+and some_dist = id
+and imp_dist_assn = "imp_dist_assn G"
+and set_all_dists_in_front_imp = set_all_dists_in_front_imp
+proof(unfold_locales, goal_cases)
+  case (1 BFS_tree frontier vis)
+  then show ?case 
+    by blast
+next
+  case (2 BFS_tree frontier vis)
+  then show ?case 
+    using expand_tree(2) by presburger
+next
+  case (3 BFS_tree frontier vis)
+  then show ?case 
+     using expand_tree(3) by presburger   
+next
+  case (4 frontier vis front' vis')
+  then show ?case 
+    using next_frontier_and_curent_correct by blast
+next
+  case (5 frontier vis front' vis')
+  then show ?case
+    using next_frontier_and_curent_correct(2)[OF _ _ 5(3,4,5,6)] by blast
+next
+  case (6 frontier vis front' vis')
+  then show ?case 
+    by force
+next
+  case (7 frontier vis front' vis')
+  then show ?case 
+    using next_frontier_and_curent_correct(4)[OF _ _ 7(3,4,5,6)] by blast
+next
+  case (8 S)
+  then show ?case 
+    by simp
+next
+  case (9 dists front S n)
+  thus ?case 
+    unfolding Vs_same by simp
+next
+  case (10 dists front S n x)
+  thus ?case 
+    by presburger
+next
+  case (11 dists front S n x)
+  thus ?case 
+    unfolding Vs_same 
+    apply(subst if_not_P)
+    by force+
+next
+  case 12
+  thus ?case 
+    by simp
+next
+  case (13 S Si)
+  then show ?case 
+    using imp_cf_is_empty_rule by fast
+next
+  case (14 S Si)
+  then show ?case 
+    by(sep_auto simp: imp_src_assn_def imp_src_to_cf_def)
+next
+  case (15 empty_vis S Si)
+  then show ?case 
+    using set_srcs_visited_rule[of G S Si empty_vis] by simp
+next
+  case (16 cf imp_cf vis imp_vis)
+  then show ?case 
+    using next_frontier_and_current_imp_rule[OF finite_Vs refl, of G cf imp_cf vis imp_vis]
+    by fast
+next 
+  case (17 vis visi s)
+  then show ?case 
+    using memb_rule[of "Vs G" "set vis" visi s] by force
+next
+  case (18 cf cfi n d id)
+  then show ?case 
+    using set_all_dists_in_front_imp_rule[of G d id cf cfi n] by force
+qed
+
+end
+end
+
+definition "barr_fixed_univ_set_assn U S Si
+       = (\<exists>\<^sub>A blist. Si \<mapsto>\<^sub>a blist * 
+             \<up> ((\<forall> u \<in> U. u < length blist \<and> blist ! u \<longleftrightarrow> (u\<in> S)) \<and> S \<subseteq> U))"
+
+interpretation imp_fixed_univ_set barr_fixed_univ_set_assn
+  apply unfold_locales 
+  apply(rule ent_iffI)
+  by(sep_auto simp: barr_fixed_univ_set_assn_def)
+
+definition "barr_fixed_univ_set_memb x S =
+     Array.nth S x"
+
+interpretation imp_fixed_univ_set_memb barr_fixed_univ_set_assn barr_fixed_univ_set_memb
+  apply unfold_locales
+  apply(sep_auto simp: barr_fixed_univ_set_assn_def barr_fixed_univ_set_memb_def)
+  subgoal for U s p a blist aa b
+    apply(rule mod_exI[of _ blist])
+    apply (sep_auto simp: mod_pure_star_dist)
+    sledgehammer
+  
+  find_theorems "_ \<Turnstile> _ * _ = _"
 
 end
